preuves de is_empty, is_full, peek_back

examples/Sek/EChunk.ml
@@ -1,51 +1,70 @@
-
-(* type 'a default = 'a*)
-
+(**
+  Type pour des buffers circulaires de capacité fixe K
+*)
 type 'a echunk = {
   data : 'a array;
   mutable front : int;
   mutable size : int;
-  default : 'a (* ['a default] *); }
+  default : 'a
+}
+let capacity = 32
 
-(* Capacity is hard-coded for now, to avoid the boilerplate of a functor *)
-let capacity = 16
+let echunk_default c = c.default
 
-let echunk_default c =
-  c.default
+let echunk_dummy d = {
+  data = [||];
+  front = 0;
+  size = 0;
+  default = d
+}
 
-let echunk_dummy d =
-  { data = [||];
-    top = 0;
-    default = d; }
+let echunk_create d = {
+  data = Array.make capacity d;
+  front = 0;
+  size = 0;
+  default = d
+}
 
-let echunk_create d =
-  { data = Array.make capacity d;
-    top = 0;
-    default = d; }
+let echunk_is_empty c = (c.size = 0)
+let echunk_is_full c = (c.size = capacity)
 
-let echunk_is_empty c =
-  c.top = 0
+let wrap_up n = if n >= capacity then n - capacity else n
 
-let echunk_is_full c =
-  c.top = capacity
+let echunk_peek_back c =
+  let back = wrap_up (c.front + c.size - 1) in
+  c.data.(back)
 
-let echunk_peek c =
-  assert (not (echunk_is_empty c));
-  c.data.(c.top-1)
-
-let echunk_pop c =
-  let x = echunk_peek c in
-  let newtop = c.top - 1 in
-  c.top <- newtop;
-  c.data.(newtop) <- c.default;
+let echunk_pop_back c =
+  let x = echunk_peek_back c in
+  let new_size = c.size - 1 in
+  c.size <- new_size;
+  let i = wrap_up (c.front + new_size) in
+  c.data.(i) <- c.default;
   x
 
-let wrap_up n = if n > capacity then n - capacity else n
-
 let echunk_push_back c x =
-  let i = wrap_up (c.front + c.size) in
-  c.data.(i) <- x;
-  c.size <- c.size + 1
+  let old_size = c.size in
+  c.size <- old_size + 1;
+  let i = wrap_up (c.front + old_size) in
+  c.data.(i) <- x
+
+let wrap_down n = if n < 0 then n + capacity else n
+
+let echunk_peek_front c = c.data.(c.front)
+
+let echunk_pop_front c =
+  let x = echunk_peek_front c in
+  let old_front = c.front in
+  c.size <- c.size - 1;
+  c.front <- wrap_up (old_front + 1);
+  c.data.(old_front) <- c.default;
+  x
+
+let echunk_push_front c x =
+  let new_front = wrap_down (c.front - 1) in
+  c.size <- c.size + 1;
+  c.front <- new_front;
+  c.data.(new_front) <- x
 
 (* let echunk_get c i =
   c.data.(i)
